## Quadratic-Equation-Frebby

####  Steps To Solving A Quadratic Equation

## Method 1 : Factorization
Let you have an equation 2x^2+5x+2=0

• To factor the equation first use factor of the x^2 term and constant term 2 then multiply them and add up with the x term.
Here 2x^2*2=4x^2 and can be written as 4x+x. 5x can also be written as 4x+x .So the equation becomes 2x^2+4x+x+2=0

• Take a common term of the equation. The equation becomes 2x(x+2)+1(x+2)=0

• Again, take common. The equation becomes (x+2)(2x+1)=0

• Set each parentheses set equal to zero. This will give you two separate equation, by solving these equation you will get x values.
(x+2)=0 or (2x+1)=0

• Solve the equation separately.
=>x+2=0
=>x=-2

And
=>2x+1=0
=>2x=-1
=>x=-1/2

• The roots of your equation are x=-2 and x= -1/2

• For cross check your answer multiply (x+2)(2x+1)=0
=>2x^2+x+4x+2=0
=>2x^2+5x+2=0

• If your equation is in the form of 2x^2+9x =-2+4x. First simplify equation the in the form of general quadratic equation.

• Take all the term one side.
=>2x^2+9x+2-4x=0

• Simplify the terms.
=>2x^2+5x+2=0

• Then follow the above steps.

## Method 2 : Using the Quadratic Formula

When it is difficult to factor the equation use quadratic formula. The quadratic equation is ax^2+bx+c=0
then the quadratic formula is:
x= [-b±v(b^2-4ac)]/[2a]

Let you have an equation x^2-6x+3=0
• Compare your equation x^2-6x+3=0 with general form ax^2+bx+c=0.

• Identify the value of a, b and c. Variable a is the coefficient of x^2, b is the coefficient of x and c is constant. Here a=1 ,b= -6 and c=3.

• Make use of formula. Substitute a, b and c values into the formula x= [-b±v(b^2-4ac)]/[2a].
=> x= [-(-6)±v(6^2-4*1*3)]/[2*1]

• Solve for x.
=>x = [6±v(36-12)]/[2]
=>x = [6±v(24)]/2
=>x = 1/2[6±2v6]
=>x = [3±v6]

• Simplify the roots.
=>x=[3+v6]
=>x=[3-v6]

Online Algebra Tutor provide you step by step explanation on Algebra topics.

## Method 3 : By Completing the Square

Completing the Square is one more method of solving quadratic equation.
Let you have an equation 2x^2-8x-9 = 0

• Take constant term right side of the equation
=>2x^2-8x = 9

• Divide both the side by the coefficient of x^2. If you have no coefficient of x^2 then just divide by 1. you can also skip this step.
=>2x^2/2-8x/2 = 9/2
=>x^2-4x = 9/2

• Divide coefficient of b by 2 then square it.
=>4/2
=>(2)^2
=>4

• Add 25/4 both sides of the equation.
=>x^2-4x+(2)^2 = 9/2+4

• Right side of the equation is in the form of (a-b)2=a2-2ab+b2.
=>(x-2)^2 = 9/2+4

• Simplify the equation.
=>(x-2)^2 = 17/2
=>(x-2)= ± v(17/2)
=>x= ± v(17/2)+2

• Roots are
=>x = 2+v(17/2)
=>x = 2-v(17/2)

Important points:

1. If x^2 or x term has no coefficient, then the coefficient is always 1.

2. If any term does exist, then the coefficient of that term will be zero.
ex. x^2+9=0
Here the coefficient of x is 0. means b=0

3. For better understanding of quadratic equation you can take help from a Online Math Tutoring.

4. You can also use quadratic calculator to find the roots of quadratic equation.
